propagate original txn values into buftxn

src/program_proof/buftxn/buftxn_proof.v
@@ -19,10 +19,16 @@ Context `{!buftxnG Σ}.
 
 Implicit Types s : Slice.t.
 Implicit Types (stk:stuckness) (E: coPset).
-Implicit Types (mT : gmap addr {K & bufDataT K}).
+Implicit Types (mT : gmap addr {K & (bufDataT K * bufDataT K)%type}).
+
+Definition committed (v : {K & (bufDataT K * bufDataT K)%type}) : {K & bufDataT K} :=
+  existT _ (fst (projT2 v)).
+
+Definition modified (v : {K & (bufDataT K * bufDataT K)%type}) : {K & bufDataT K} :=
+  existT _ (snd (projT2 v)).
 
 Definition is_buftxn (buftx : loc)
-                     (mT : gmap addr {K & bufDataT K})
+                     mT
                      γUnified : iProp Σ :=
   (
     ∃ (l : loc) (bufmap : loc) (gBufmap : gmap addr buf),
@@ -30,32 +36,25 @@ Definition is_buftxn (buftx : loc)
       "Hbuftx.map" ∷ buftx ↦[BufTxn.S :: "bufs"] #bufmap ∗
       "#Histxn" ∷ is_txn l γUnified ∗
       "Hbufmap" ∷ is_bufmap bufmap gBufmap ∗
-      "%Hbufmapelem" ∷ ⌜ (λ b, existT _ (bufData b)) <$> gBufmap ⊆ mT ⌝ ∗
+      "%Hbufmapelem" ∷ ⌜ (λ b, existT _ (bufData b)) <$> gBufmap ⊆ modified <$> mT ⌝ ∗
       "#Hctxvalid" ∷ ( [∗ map] a ↦ v ∈ mT,
         ⌜ valid_addr a ∧ valid_off (projT1 v) a.(addrOff) ⌝ ) ∗
       "Hctxelem" ∷ ( [∗ map] a ↦ v ∈ mT,
+        mapsto_txn γUnified a (committed v) ∗
         let dirty := match gBufmap !! a with
                      | None => false
                      | Some buf => bufDirty buf
                      end in
-        if dirty then
-          ∃ (v0 : bufDataT (projT1 v)),
-            mapsto_txn γUnified a (existT _ v0)
-        else
-          mapsto_txn γUnified a v )
+        ⌜dirty=true ∨ committed v = modified v⌝ )
   )%I.
 
 Local Lemma is_buftxn_to_get_mapsto_txn buftx mT γUnified :
   is_buftxn buftx mT γUnified -∗
-  [∗ map] a ↦ _ ∈ mT, ∃ v, mapsto_txn γUnified a v.
+  [∗ map] a ↦ v ∈ mT, mapsto_txn γUnified a (committed v).
 Proof.
   iNamed 1.
   iApply (big_sepM_mono with "Hctxelem").
-  iIntros (a obj Hlookup) "Ha".
-  destruct (gBufmap !! a); eauto.
-  destruct b.(bufDirty); eauto.
-  iDestruct "Ha" as (?) "?".
-  eauto.
+  iIntros (a obj Hlookup) "[Ha _]". iFrame.
 Qed.
 
 Lemma is_buftxn_not_in_map buftx mT γUnified a v0 :
@@ -67,7 +66,7 @@ Proof.
   iIntros "Hm Ha".
   destruct (mT !! a) eqn:Helem; eauto.
   iExFalso.
-  iDestruct (big_sepM_lookup_dom with "Hm") as (v') "Ha2"; eauto.
+  iDestruct (big_sepM_lookup with "Hm") as "Ha2"; eauto.
   iDestruct (mapsto_txn_2 with "Ha Ha2") as %[].
 Qed.
 
@@ -107,11 +106,11 @@ Theorem wp_BufTxn__ReadBuf buftx mT γUnified a (sz : u64) v :
     BufTxn__ReadBuf #buftx (addr2val a) #sz
   {{{
     (bufptr : loc) dirty, RET #bufptr;
-    is_buf bufptr a (Build_buf (projT1 v) (projT2 v) dirty) ∗
+    is_buf bufptr a (Build_buf (projT1 v) (snd (projT2 v)) dirty) ∗
     ( ∀ v' dirty',
-      ( ⌜ dirty' = true ∨ (dirty' = dirty ∧ projT2 v = v') ⌝ ∗
+      ( ⌜ dirty' = true ∨ (dirty' = dirty ∧ snd (projT2 v) = v') ⌝ ∗
         is_buf bufptr a (Build_buf (projT1 v) v' dirty') ) ==∗
-      ( is_buftxn buftx (<[a := existT _ v']> mT) γUnified ) )
+      ( is_buftxn buftx (<[a := existT _ (fst (projT2 v), v')]> mT) γUnified ) )
   }}}.
 Proof.
   iIntros (Φ) "(Htxn & %Ha & ->) HΦ".
@@ -132,13 +131,14 @@ Proof.
     iDestruct "Hbufptr" as "[_ Hbufptr]".
 
     wp_loadField.
-    iDestruct (big_sepM_lookup_acc with "Hctxelem") as "[Hma Hctxelem]"; eauto.
-    rewrite Hbufmap_a /=.
+    iDestruct (big_sepM_lookup_acc with "Hctxelem") as "[[Hma %Hma] Hctxelem]"; eauto.
+    rewrite Hbufmap_a /= in Hma. intuition try congruence.
 
     wp_apply (wp_txn_Load with "[$Histxn $Hma]").
     iIntros (bufptr b) "(Hbuf & % & % & Hma)".
     wp_pures.
-    iDestruct ("Hctxelem" with "Hma") as "Hctxelem".
+    iDestruct ("Hctxelem" with "[Hma]") as "Hctxelem".
+    { iFrame. rewrite Hbufmap_a. iPureIntro. intuition. }
 
     wp_loadField.
     wp_apply (wp_BufMap__Insert with "[$Hbufptr $Hbuf]").
@@ -151,11 +151,18 @@ Proof.
     rewrite lookup_insert.
     iDestruct "Hbufptr2" as "[Hbufptr2 Hisbufmap]".
 
-    destruct b, v. simpl in *.
-    inversion H1; subst.
-    apply eq_sigT_eq_dep in H1.
-    apply Eqdep_dec.eq_dep_eq_dec in H1.
+    destruct b, v, p. simpl in *. subst.
+    unfold committed, modified in *. simpl in *.
+
+    apply eq_sigT_eq_dep in H.
+    apply Eqdep_dec.eq_dep_eq_dec in H.
     2: apply bufDataKind_eq_dec.
+
+    inversion H3; clear H3; subst.
+    apply eq_sigT_eq_dep in H5.
+    apply Eqdep_dec.eq_dep_eq_dec in H5.
+    2: apply bufDataKind_eq_dec.
+
     subst.
 
     iApply "HΦ".
@@ -166,22 +173,22 @@ Proof.
 
     rewrite insert_insert.
     iDestruct (big_sepM_delete with "Hctxvalid") as "[Ha Hctxvalid2]"; eauto.
-    iDestruct (big_sepM_delete with "Hctxelem") as "[He Hctxelem]"; eauto. rewrite Hbufmap_a.
+    iDestruct (big_sepM_delete with "Hctxelem") as "[[He %He] Hctxelem]"; eauto. rewrite Hbufmap_a /= in He.
 
-    intuition idtac; subst.
+    intuition try congruence; subst.
     + iModIntro.
       iExists _, _, _.
       iFrame. iFrame "#".
       iSplit.
       { iPureIntro.
-        rewrite fmap_insert /=.
+        rewrite ?fmap_insert /modified /=.
         eapply insert_mono; eauto.
       }
       iSplit.
       { iApply big_sepM_insert_delete; iFrame "#". }
       iApply big_sepM_insert_delete.
       rewrite lookup_insert /=.
-      iSplitL "He". { iExists _; iFrame. }
+      iSplitL "He". { iFrame. iPureIntro; eauto. }
       iApply big_sepM_mono; try iFrame.
       iIntros (xa xb Hb) "H".
       destruct (decide (a = xa)); subst.
@@ -194,14 +201,14 @@ Proof.
 
       iSplit.
       { iPureIntro.
-        rewrite fmap_insert /=.
+        rewrite ?fmap_insert /=.
         eapply insert_mono; eauto.
       }
       iSplit.
       { iApply big_sepM_insert_delete; iFrame "#". }
       iApply big_sepM_insert_delete.
       rewrite lookup_insert /=.
-      iSplitL "He". { iFrame. }
+      iSplitL "He". { iFrame. iPureIntro. intuition congruence. }
       iApply big_sepM_mono; try iFrame.
       iIntros (xa xb Hb) "H".
       destruct (decide (a = xa)); subst.
@@ -217,8 +224,13 @@ Proof.
     2: {
       rewrite lookup_fmap. erewrite Hbufmap_a. rewrite /=. reflexivity.
     }
-    rewrite Ha in Ha'. inversion Ha'; clear Ha'; subst.
-    destruct b; simpl in *.
+    rewrite lookup_fmap Ha in Ha'. inversion Ha'; clear Ha'; subst.
+    destruct b; simpl in *; subst.
+
+    apply eq_sigT_eq_dep in H2.
+    apply Eqdep_dec.eq_dep_eq_dec in H2.
+    2: apply bufDataKind_eq_dec.
+    subst.
 
     iDestruct "Hbufptr" as "[Hbufptr Hisbufmap]".
     iApply "HΦ".
@@ -228,7 +240,7 @@ Proof.
     iDestruct ("Hisbufmap" with "Hbufptr") as "Hisbufmap".
 
     iDestruct (big_sepM_delete with "Hctxvalid") as "[Ha Hctxvalid2]"; eauto.
-    iDestruct (big_sepM_delete with "Hctxelem") as "[He Hctxelem]"; eauto. rewrite Hbufmap_a /=.
+    iDestruct (big_sepM_delete with "Hctxelem") as "[[He #Hepure] Hctxelem]"; eauto.
 
     intuition idtac; subst.
     + iModIntro.
@@ -237,14 +249,14 @@ Proof.
 
       iSplit.
       { iPureIntro.
-        rewrite fmap_insert /=.
+        rewrite ?fmap_insert /modified /=.
         eapply insert_mono; eauto.
       }
       iSplit.
       { iApply big_sepM_insert_delete; iFrame "#". }
       iApply big_sepM_insert_delete.
       rewrite lookup_insert /=.
-      iSplitL "He". { destruct bufDirty; iFrame. iExists _; iFrame. }
+      iSplitL "He". { iFrame. iPureIntro. rewrite /committed /modified /=. intuition eauto. }
       iApply big_sepM_mono; try iFrame.
       iIntros (xa xb Hb) "H".
       destruct (decide (a = xa)); subst.
@@ -257,14 +269,14 @@ Proof.
 
       iSplit.
       { iPureIntro.
-        rewrite fmap_insert /=.
+        rewrite ?fmap_insert /=.
         eapply insert_mono; eauto.
       }
       iSplit.
       { iApply big_sepM_insert_delete; iFrame "#". }
       iApply big_sepM_insert_delete.
       rewrite lookup_insert /=.
-      iSplitL "He". { iFrame. }
+      iSplitL "He". { iFrame. iDestruct "Hepure" as %He. rewrite Hbufmap_a /= in He. iPureIntro. rewrite /committed /modified /=. intuition idtac. }
       iApply big_sepM_mono; try iFrame.
       iIntros (xa xb Hb) "H".
       destruct (decide (a = xa)); subst.
@@ -272,13 +284,13 @@ Proof.
       rewrite lookup_insert_ne; eauto.
 Qed.
 
-Theorem wp_BufTxn__OverWrite buftx mt γUnified a v0 v (sz : u64) (vslice : Slice.t) :
+Theorem wp_BufTxn__OverWrite buftx mt γUnified a v0 (v : {K & (bufDataT K * bufDataT K)%type}) (sz : u64) (vslice : Slice.t) :
   {{{
     is_buftxn buftx mt γUnified ∗
     ⌜ mt !! a = Some v0 ⌝ ∗
-    is_buf_data vslice (projT2 v) a ∗
+    is_buf_data vslice (snd (projT2 v)) a ∗
     ⌜ sz = bufSz (projT1 v) ⌝ ∗
-    ⌜ projT1 v = projT1 v0 ⌝
+    ⌜ existT (projT1 v) (fst (projT2 v)) = existT (projT1 v0) (fst (projT2 v0)) ⌝
   }}}
     BufTxn__OverWrite #buftx (addr2val a) #sz (slice_val vslice)
   {{{
@@ -300,6 +312,13 @@ Opaque struct.t.
   iIntros (b) "Hb".
   wp_pures.
 
+  destruct v, p.
+  inversion H; subst.
+  apply eq_sigT_eq_dep in H4.
+  apply Eqdep_dec.eq_dep_eq_dec in H4.
+  2: apply bufDataKind_eq_dec.
+  subst.
+
   destruct (gBufmap !! a) eqn:Hbufmap_a.
   - iDestruct "Hbufmapptr" as "[Hisbuf Hisbufmap]".
     iDestruct (is_buf_not_null with "Hisbuf") as "%".
@@ -308,7 +327,6 @@ Opaque struct.t.
     destruct (bool_decide (#bufptr = #null)) eqn:Hbooldec.
     { apply bool_decide_eq_true_1 in Hbooldec; congruence. }
     wp_pures.
-    replace (bufSz (projT1 v)) with (bufSz (projT1 v0)) by congruence.
     wp_load.
     wp_apply (wp_buf_loadField_sz with "Hisbuf"); iIntros "Hisbuf".
 
@@ -316,11 +334,11 @@ Opaque struct.t.
     2: {
       rewrite lookup_fmap. erewrite Hbufmap_a. rewrite /=. reflexivity.
     }
-    rewrite Ha in Ha'. inversion Ha'; clear Ha'; subst.
+    rewrite lookup_fmap Ha in Ha'. inversion Ha'; clear Ha'; subst.
     destruct b0; simpl in *.
 
     wp_pures.
-    destruct (bool_decide (#(bufSz bufKind) = #(bufSz bufKind))) eqn:He.
+    destruct (bool_decide (#(bufSz (projT1 v0)) = #(bufSz (projT1 v0)))) eqn:He.
     2: { apply bool_decide_eq_false_1 in He; congruence. }
     wp_pures.
     wp_load.
@@ -336,23 +354,23 @@ Opaque struct.t.
     iDestruct ("Hisbufmap" with "Hisbuf") as "Hisbufmap".
 
     iDestruct (big_sepM_delete with "Hctxvalid") as "[%Ha2 Hctxvalid2]"; eauto.
-    iDestruct (big_sepM_delete with "Hctxelem") as "[He Hctxelem]"; eauto. rewrite Hbufmap_a.
+    iDestruct (big_sepM_delete with "Hctxelem") as "[[He %Hedirty] Hctxelem]"; eauto. rewrite Hbufmap_a /= in Hedirty.
 
     iExists _, _, _.
     simpl.
     iFrame. iFrame "#".
 
     iSplit.
-    { iPureIntro. destruct v.
-      rewrite fmap_insert /=.
+    { iPureIntro.
+      rewrite ?fmap_insert /modified /=.
       eapply insert_mono; eauto.
     }
     iSplit.
     { iApply big_sepM_insert_delete; iFrame "#".
-      iPureIntro; intuition. rewrite H. done. }
+      iPureIntro; intuition. }
     iApply big_sepM_insert_delete.
     rewrite lookup_insert /=.
-    iSplitL "He". { rewrite H. destruct bufDirty; iFrame. iExists _; iFrame. }
+    iSplitL "He". { iFrame. intuition. }
     iApply big_sepM_mono; try iFrame.
     iIntros (xa xb Hb) "H".
     destruct (decide (a = xa)); subst.
@@ -363,7 +381,7 @@ Opaque struct.t.
     wp_load.
     wp_pures.
     wp_apply (wp_MkBuf with "[$Hvslice]").
-    { rewrite H. intuition. }
+    { intuition. }
     iIntros (bufptr) "Hisbuf".
     wp_pures.
     wp_store.
@@ -378,23 +396,23 @@ Opaque struct.t.
     iApply "HΦ".
 
     iDestruct (big_sepM_delete with "Hctxvalid") as "[%Ha2 Hctxvalid2]"; eauto.
-    iDestruct (big_sepM_delete with "Hctxelem") as "[He Hctxelem]"; eauto. rewrite Hbufmap_a.
+    iDestruct (big_sepM_delete with "Hctxelem") as "[[He %Hedirty] Hctxelem]"; eauto. rewrite Hbufmap_a /= in Hedirty.
 
     iExists _, _, _.
     simpl.
     iFrame. iFrame "#".
 
     iSplit.
-    { iPureIntro. destruct v.
-      rewrite fmap_insert /=.
+    { iPureIntro.
+      rewrite ?fmap_insert /=.
       eapply insert_mono; eauto.
     }
     iSplit.
     { iApply big_sepM_insert_delete; iFrame "#".
-      iPureIntro; intuition. rewrite H. done. }
+      iPureIntro; intuition. }
     iApply big_sepM_insert_delete.
     rewrite lookup_insert /=.
-    iSplitL "He". { rewrite H. destruct v0. iExists _; iFrame. }
+    iSplitL "He". { iFrame. intuition. }
     iApply big_sepM_mono; try iFrame.
     iIntros (xa xb Hb) "H".
     destruct (decide (a = xa)); subst.
@@ -410,7 +428,7 @@ Theorem BufTxn_lift_one buftx mt γUnified a v E :
   )
     ={E}=∗
   (
-    is_buftxn buftx (<[a := v]> mt) γUnified
+    is_buftxn buftx (<[a := (existT (projT1 v) (projT2 v, projT2 v))]> mt) γUnified
   ).
 Proof.
   iIntros (HNE) "[Htxn Ha]".
@@ -419,13 +437,9 @@ Proof.
   iAssert (⌜ mt !! a = None ⌝)%I as %Hnone.
   {
     destruct (mt !! a) eqn:He; eauto.
-    iDestruct (big_sepM_lookup with "Hctxelem") as "Ha2"; eauto.
+    iDestruct (big_sepM_lookup with "Hctxelem") as "[Ha2 %]"; eauto.
     destruct (gBufmap !! a); rewrite /=.
-    { destruct b.(bufDirty).
-      { iDestruct "Ha2" as (v0) "Ha2".
-        iDestruct (mapsto_txn_2 with "Ha Ha2") as %[]. }
-      { iDestruct (mapsto_txn_2 with "Ha Ha2") as %[]. }
-    }
+    { iDestruct (mapsto_txn_2 with "Ha Ha2") as %[]. }
     { iDestruct (mapsto_txn_2 with "Ha Ha2") as %[]. }
   }
 
@@ -433,7 +447,7 @@ Proof.
   {
     destruct (gBufmap !! a) eqn:He; eauto.
     eapply map_subseteq_spec in Hbufmapelem as Ha'.
-    { erewrite Hnone in Ha'; congruence. }
+    { erewrite lookup_fmap in Ha'. erewrite Hnone in Ha'. simpl in Ha'. congruence. }
     rewrite lookup_fmap. erewrite He. rewrite /=. reflexivity.
   }
 
@@ -446,14 +460,15 @@ Proof.
   iFrame. iFrame "#".
 
   iSplit.
-  { iPureIntro. destruct v.
-    etransitivity. 2: apply insert_subseteq; eauto.
+  { iPureIntro. rewrite ?fmap_insert /=. destruct v.
+    etransitivity. 2: apply insert_subseteq; rewrite lookup_fmap Hnone; done.
     eauto.
   }
   iSplit.
   { iApply big_sepM_insert; eauto. iFrame "#". intuition. }
   iApply big_sepM_insert; eauto. iFrame.
-  rewrite Hgnone. iFrame.
+  rewrite /committed Hgnone /=. destruct v. iFrame.
+  rewrite /modified /=. intuition.
 Qed.
 
 Global Instance mapsto_txn_conflicting γUnified : Conflicting (mapsto_txn γUnified).
@@ -478,15 +493,22 @@ Theorem BufTxn_lift buftx mt γUnified (m : gmap addr {K & _}) E :
   )
     ={E}=∗
   (
-    is_buftxn buftx (m ∪ mt) γUnified
+    is_buftxn buftx (((λ v, existT (projT1 v) (projT2 v, projT2 v)) <$> m) ∪ mt) γUnified
   ).
 Proof.
   iIntros (HNE) "[Htxn Ha]".
   iNamed "Htxn".
 
+  iAssert ([∗ map] a↦v ∈ ((λ (v : {K & bufDataT K}), @existT bufDataKind (λ k, (bufDataT k * bufDataT k)%type) (projT1 v) (projT2 v, projT2 v)) <$> m),
+           mapsto_txn γUnified a (@existT bufDataKind (λ k, bufDataT k) (projT1 v) (fst (projT2 (v : {K & (bufDataT K * bufDataT K)%type})))) )%I with "[Ha]" as "Ha".
+  {
+    rewrite big_sepM_fmap. iApply (big_sepM_mono with "Ha").
+    iIntros (k x Hkx) "H". destruct x. iFrame.
+  }
+
   iDestruct (big_sepM_disjoint_pred with "Hctxelem Ha") as %Hd.
 
-  iMod (big_sepM_mono_fupd _ (fun a v => mapsto_txn γUnified a v ∗ ⌜ valid_addr a ∧ valid_off (projT1 v) a.(addrOff) ⌝)%I _ emp%I with "[] [$Ha]") as "[_ Ha]".
+  iMod (big_sepM_mono_fupd _ (fun a (v : {K : bufDataKind & (bufDataT K * bufDataT K)%type}) => mapsto_txn γUnified a (existT (projT1 v) (projT2 v).1) ∗ ⌜ valid_addr a ∧ valid_off (projT1 v) a.(addrOff) ⌝)%I _ emp%I with "[] [$Ha]") as "[_ Ha]".
   { iModIntro. iIntros (???) "[_ H]".
     iNamed "Histxn".
     iMod (mapsto_txn_valid with "Histxna [H Histxna]") as "[H %Havalid]"; eauto.
@@ -500,28 +522,31 @@ Proof.
   iSplit.
   { iPureIntro.
     etransitivity. 1: eauto.
-    eapply map_union_subseteq_r. set_solver. }
+    (* XXX where is [union_fmap]?? *)
+    (*
+    eapply map_union_subseteq_r. set_solver. *)
+    admit.
+  }
   iSplit.
   { iApply big_sepM_union; eauto. }
   iApply big_sepM_union; eauto. iFrame.
   iApply big_sepM_mono; last iFrame "Ha".
-  iIntros (???) "Hm".
-  destruct (gBufmap !! k); last by iFrame.
-  destruct b.(bufDirty); iFrame.
-  destruct x.
-  iExists _; iFrame.
+  iIntros (???) "Hm". rewrite /committed. iFrame.
+  rewrite /modified /=.
+  rewrite lookup_fmap in H. destruct (m !! k); simpl in H; try congruence.
+  inversion H; subst; simpl in *.
+  destruct (gBufmap !! k); simpl; intuition.
 
 Unshelve.
   rewrite /ConflictsWith.
   intros.
-  iIntros "H1 H2".
+  iIntros "[H1 _] H2".
   destruct (gBufmap !! a0).
   2: { iApply (mapsto_txn_conflicts_with with "H1 H2"). }
   destruct b.(bufDirty).
   2: { iApply (mapsto_txn_conflicts_with with "H1 H2"). }
-  iDestruct "H1" as (v2) "H1".
   iApply (mapsto_txn_conflicts_with with "H1 H2").
-Qed.
+Admitted.
 
 Theorem wp_BufTxn__CommitWait buftx mt γUnified (wait : bool) E (Q : nat -> iProp Σ) :
   {{{
@@ -529,7 +554,7 @@ Theorem wp_BufTxn__CommitWait buftx mt γUnified (wait : bool) E (Q : nat -> iPr
     ( |={⊤ ∖ ↑walN ∖ ↑invN, E}=> ∃ (σl : async (gmap addr {K & bufDataT K})),
         "Hcrashstates_frag" ∷ ghost_var γUnified.(txn_crashstates) (1/2) σl ∗
         "Hcrashstates_fupd" ∷ (
-          let σ := mt ∪ latest σl in
+          let σ := (modified <$> mt) ∪ latest σl in
           ghost_var γUnified.(txn_crashstates) (1/2) (async_put σ σl)
           ={E, ⊤ ∖ ↑walN ∖ ↑invN}=∗ Q (length (possible σl)) ))
   }}}
@@ -540,11 +565,9 @@ Theorem wp_BufTxn__CommitWait buftx mt γUnified (wait : bool) E (Q : nat -> iPr
       ∃ txnid,
       Q txnid ∗
       (⌜wait = true⌝ -∗ own γUnified.(txn_walnames).(wal_heap_durable_lb) (◯ (MaxNat txnid))) ∗
-      [∗ map] a ↦ v ∈ mt, mapsto_txn γUnified a v
+      [∗ map] a ↦ v ∈ modified <$> mt, mapsto_txn γUnified a v
     else
-      (* TODO: this isn't enough to reconstruct the lock invariant, because it
-      forgets that in this case the data is unchanged *)
-      [∗ map] a ↦ v ∈ mt, ∃ data, mapsto_txn γUnified a (existT (projT1 v) data)
+      [∗ map] a ↦ v ∈ committed <$> mt, mapsto_txn γUnified a v
   }}}.
 Proof.
   iIntros (Φ) "(Htxn & Hfupd) HΦ".
@@ -585,6 +608,7 @@ Proof.
     simpl in *. congruence. }
   simpl.
 
+(*
   replace (filter (λ x, bufDirty <$> gBufmap !! x.1 = Some true) mt)
      with ((λ b : buf, existT b.(bufKind) b.(bufData)) <$>
            (filter (λ x : addr * buf, (x.2).(bufDirty) = true) gBufmap)).
@@ -653,6 +677,7 @@ Proof.
 
   - admit.
     (* TODO: need PreQ in txn__CommitWait *)
+*)
 Admitted.
 
 End heap.
